Surface/Ty/Definition.lean
@@ -1,12 +1,17 @@
+import Core.Vec
+import Lilac
+open Lilac
 
-inductive Surface.BaseKind : Type where
+namespace Surface
+
+inductive BaseKind : Type where
 | closed
 | «open»
 
 notation "b`★" => Surface.BaseKind.closed
 notation "b`◯" => Surface.BaseKind.open
 
-inductive Surface.Kind : Type where
+inductive Kind : Type where
 | base : BaseKind -> Kind
 | arrow : Kind -> Kind -> Kind
 
@@ -14,7 +19,7 @@ notation "`★" => Surface.Kind.base Surface.BaseKind.closed
 notation "`◯" => Surface.Kind.base Surface.BaseKind.open
 infixr:64 " `-:> " => Surface.Kind.arrow
 
-inductive Surface.Ty : Type where
+inductive Ty : Type where
 | var : Nat -> Ty
 | global : String -> Ty
 | arrow : Ty -> Ty -> Ty
@@ -22,7 +27,15 @@ inductive Surface.Ty : Type where
 | all : Kind -> Ty -> Ty
 | app : Ty -> Ty -> Ty
 
-def Surface.Ty.size : Ty -> Nat
+-- Us -> Es -> Ts -> R
+-- Us = "Universally quantified" types, will be applied in a pattern
+-- Es = "Existentionally quantified" types, will be bound by a pattern
+-- Ts = Subdata, will be bound by a pattern
+-- R = Return type (datatype for constructors, anything for an open method)
+abbrev SpineTy := (m1 : Nat) × Vec Kind m1 × (m2 : Nat) × Vec Kind m2 × (n : Nat) × Vec Ty n × Ty
+
+
+def Ty.size : Ty -> Nat
 | var _ => 0
 | global _ => 0
 | all _ t => t.size + 1
@@ -30,7 +43,7 @@ def Surface.Ty.size : Ty -> Nat
 | «then» t1 t2 => t1.size + t2.size + 1
 | app t1 t2 => t1.size + t2.size + 1
 
-instance Surface.instSizeOf_Ty : SizeOf Surface.Ty where
+instance instSizeOf_Ty : SizeOf Surface.Ty where
   sizeOf := Surface.Ty.size
 
 prefix:max "t`#" => Surface.Ty.var
@@ -40,7 +53,7 @@ infixr:64 " `=:> " => Surface.Ty.then
 notation "`∀[" K "]" B => Surface.Ty.all K B
 infixl:54 " `• " => Surface.Ty.app
 
-protected def Surface.Kind.repr (p : Nat) : (a : Kind) -> Std.Format
+protected def Kind.repr (p : Nat) : (a : Kind) -> Std.Format
 | base .closed => "`★"
 | base .open => "`◯"
 | arrow k1 k2 => Repr.addAppParen ((Kind.repr max_prec k1) ++ " `-:> " ++ Kind.repr p k2) p
@@ -48,7 +61,7 @@ protected def Surface.Kind.repr (p : Nat) : (a : Kind) -> Std.Format
 instance Surface.kindRepr : Repr Surface.Kind where
   reprPrec a p := Surface.Kind.repr p a
 
-protected def Surface.Ty.repr (p : Nat) : (a : Ty) -> Std.Format
+protected def Ty.repr (p : Nat) : (a : Ty) -> Std.Format
 | var n => "t`#" ++ Nat.repr n
 | global s => "gt`#" ++ s
 | arrow t1 t2 => Repr.addAppParen (Ty.repr max_prec t1 ++ " `-:> " ++ Ty.repr p t2) p
@@ -56,8 +69,8 @@ protected def Surface.Ty.repr (p : Nat) : (a : Ty) -> Std.Format
 | all K t => Repr.addAppParen ("`∀[ " ++ repr K ++ " ] " ++ Ty.repr max_prec t) p
 | app t1 t2 => Repr.addAppParen (Ty.repr p t1 ++ " `• " ++ Ty.repr max_prec t2) p
 
-instance Surface.tyRepr : Repr Surface.Ty where
-  reprPrec a p := Surface.Ty.repr p a
+instance tyRepr : Repr Ty where
+  reprPrec a p := Ty.repr p a
 
 
 /-
@@ -69,3 +82,5 @@ case app => sorry
 case all => sorry
 
 -/
+
+end Surface
