Surface/Ty/Structure.lean
@@ -5,144 +5,124 @@ import Surface.Ty.BEq
 import Core.Util
 
 open LeanSubst
+namespace Surface
 
-def Surface.Ty.spine : Ty -> Option (String × List Ty)
+def Ty.spine : Ty -> Option (String × List Ty)
 | gt`#x => return (x, [])
 | app f a => do
   let (x, sp) <- spine f
   (x, sp ++ [a])
 | _ => none
 
-def Surface.Ty.apply (t : Ty) : List Ty -> Ty
-| [] => t
-| .cons a tl => (t `• a).apply tl
+@[simp, grind =]
+theorem Ty.spine_arrow {A B : Ty} : (A `-:> B).spine = none := by simp [spine]
 
-def Surface.Ty.arity : Ty -> Nat
-| arrow _ B => B.arity + 1
-| `∀[_] P => P.arity + 1
-| _ => 0
+@[simp, grind =]
+theorem Ty.spine_all : (`∀[K] A).spine = none := by simp [spine]
 
-inductive Surface.TeleElem
-| kind (K : Surface.Kind)
-| ty (A : Surface.Ty)
-| pred (A: Surface.Ty)
-deriving Repr
+@[simp, grind =]
+theorem Ty.spine_then : (A `=:> B).spine = none := by simp [spine]
 
-def Surface.Telescope := List Surface.TeleElem
-
-def Surface.Telescope.extend (Γ : List Surface.Ty): Telescope -> List Surface.Ty
-| [] => Γ
-| .cons (.kind _) te => extend Γ te
-| .cons (.ty A) te => extend (A::Γ) te
-| .cons (.pred A) te => extend (A::Γ) te
-
-def Surface.Telescope.rmap (r : Ren) : Telescope -> Telescope
-| [] => []
-| .cons (.kind K) te => .cons (.kind K) (rmap r te)
-| .cons (.ty A) te => .cons (.ty A[r]) (rmap r.lift te)
-| .cons (.pred A) te => .cons (.pred A[r]) (rmap r.lift te)
-
-instance Surface.instRenMap_Telescope : RenMap Surface.Telescope where
-  rmap := Surface.Telescope.rmap
-
-def Surface.Telescope.smap (σ : Subst Surface.Ty) : Surface.Telescope -> Surface.Telescope
-| [] => []
-| .cons (.kind K) te => .cons (.kind K) (smap σ te)
-| .cons (.ty A) te => .cons (.ty A[σ]) (smap σ.lift te)
-| .cons (.pred A) te => .cons (.pred A[σ]) (smap σ.lift te)
-
-instance Surface.instRenMap_TelescopeTy : SubstMap Surface.Telescope Surface.Ty where
-  smap := Surface.Telescope.smap
-
-def Surface.Ty.telescope : Ty -> Telescope  × Ty
-| .arrow A B =>
-  let (tys, b) := B.telescope
-  (.ty A :: tys, b)
-| «then» A B =>
-  let (tys, b) := B.telescope
-  (.ty A :: tys, b)
-| .all K B =>
-  let (tys, b) := B.telescope
-  (.kind K :: tys, b)
-| t => ([], t)
-
-def Surface.Telescope.count_binders (t : Surface.Telescope) : Nat :=
-  t.foldl (λ acc x => match x with
-                  | .kind _ => acc + 1
-                  | _ => acc) 0
-
-def Surface.Ty.from_telescope : List Surface.TeleElem -> Ty -> Ty
-| .nil , t => t
-| .cons (.ty A) tys, t =>
-  let r := t.from_telescope tys
-  A `-:> r
-| .cons (.pred A) tys, t =>
-  let r := t.from_telescope tys
-  A `=:> r
-| .cons (.kind K) tys, t =>
-  let r := t.from_telescope tys
-  `∀[K] r
-
-@[simp]
-theorem Surface.Ty.Spine.apply_subst {t : Ty} {sp : List Ty} : (t.apply sp)[σ] = (t[σ]).apply (sp.map (·[σ])) := by
-  induction sp generalizing t <;> simp [Surface.Ty.apply]
-  case cons hd tl ih => replace ih := @ih (t  `• hd); simp at ih; rw [ih]
-
-@[simp]
-theorem Surface.Ty.Spine.app_eq :
-  (f `• a).spine = some (x, sp)
-  <-> ∃ sp', sp = sp' ++ [a] ∧ f.spine = some (x, sp')
-:= by
-  apply Iff.intro <;> intro h
-  case _ =>
-    simp [Surface.Ty.spine] at h
-    rw [Option.bind_eq_some_iff] at h
-    rcases h with ⟨q, e1, e2⟩
-    rcases q with ⟨y, sp'⟩; simp at e2
-    rcases e2 with ⟨e2, e3⟩; subst e2 e3
-    rw [e1]; exists sp'
-  case _ =>
-    rcases h with ⟨sp', e1, e2⟩; subst e1
-    simp [Surface.Ty.spine]
-    rw [Option.bind_eq_some_iff]; apply Exists.intro (x, sp')
-    apply And.intro e2; simp
-
-theorem Surface.Ty.Spine.apply_type {t : Ty} : t.apply sp `• a = t.apply (sp ++ [a]) := by
-  induction sp generalizing t <;> simp [Surface.Ty.apply]
-  case cons hd tl ih => rw [ih]
-
-theorem Surface.Ty.Spine.apply_eq
-  : t.spine = some (x, sp) -> t = (gt`#x).apply sp
+theorem Ty.spine_subst {R : Ty} (σ : Subst Ty)
+  : R.spine = some (x, sp) -> R[σ].spine = some (x, sp[σ])
 := by
   intro h
-  fun_induction Surface.Ty.spine generalizing x sp <;> simp at *
-  case _ y =>
-    rcases h with ⟨e1, e2⟩; subst e1 e2
-    simp [Surface.Ty.apply]
+  fun_induction Ty.spine generalizing x sp
+  case _ => simp at h; rcases h with ⟨e1, e2⟩; subst e1; subst e2; simp [Ty.spine]
   case _ ih =>
-    rw [Option.bind_eq_some_iff] at h
-    rcases h with ⟨q, e1, e2⟩
-    rcases q with ⟨y, sp'⟩; simp at e2
-    rcases e2 with ⟨e2, e3⟩; subst e2 e3
-    rw [ih e1, apply_type]
+    simp at h; rw[Option.bind_eq_some_iff] at h; rcases h with ⟨⟨x', sp'⟩, h2, h⟩
+    simp at h; replace ih := ih h2
+    simp[Ty.spine]; rw[Option.bind_eq_some_iff];
+    exists (x', sp'[σ]); simp;
+    apply And.intro
+    · apply ih
+    · apply And.intro;
+      · apply h.1
+      · rw[<-h.2]; simp
+  cases h
 
-theorem Surface.Ty.Spine.apply_compose {t : Ty}
-  : t.spine = some (x, sp1) -> (t.apply sp2).spine = some (x, sp1 ++ sp2)
+theorem Ty.spine_subst {R : Ty} (σ : Subst Ty)
+  : R.spine = some (x, sp) -> R[σ].spine = some (x, sp[σ])
 := by
-  intro h; induction sp2 generalizing t x sp1
-  simp [Surface.Ty.apply]; exact h
-  case _ a tl ih =>
-  have lem : (t `• a).spine = some (x, sp1 ++ [a]) := by simp; exact h
-  replace ih := ih lem; simp at ih; exact ih
+  intro h
+  fun_induction Ty.spine generalizing x sp
+  case _ => simp at h; rcases h with ⟨e1, e2⟩; subst e1; subst e2; simp [Ty.spine]
+  case _ ih =>
+    simp at h; rw[Option.bind_eq_some_iff] at h; rcases h with ⟨⟨x', sp'⟩, h2, h⟩
+    simp at h; replace ih := ih h2
+    simp[Ty.spine]; rw[Option.bind_eq_some_iff];
+    exists (x', sp'[σ]); simp;
+    apply And.intro
+    · apply ih
+    · apply And.intro;
+      · apply h.1
+      · rw[<-h.2]; simp
+  cases h
 
-@[simp]
-theorem Surface.Ty.Spine.apply_eta : ((gt`#x).apply sp).spine = some (x, sp) := by
-  have lem := @apply_compose x [] sp gt`#x (by simp [Surface.Ty.spine])
-  simp at lem; exact lem
+theorem Ty.spine_ren {R : Ty} (r : Ren Ty)
+  : R.spine = some (x, sp) -> R⟨r⟩.spine = some (x, sp⟨r⟩)
+:= by
+  intro h
+  fun_induction Ty.spine generalizing x sp <;> simp [spine] at *
+  case _ =>
+    rcases h with ⟨h1, h2⟩; subst h1; subst h2; simp
+  case _ ih =>
+    rw[Option.bind_eq_some_iff] at h; rcases h with ⟨⟨x', sp'⟩, h2, h⟩
+    simp at h; rcases h with ⟨e1, e2⟩; subst e1; subst e2;
+    rw[Option.bind_eq_some_iff];
+    replace ih := ih h2
+    exists (x', sp'⟨r⟩)
+    apply And.intro
+    · apply ih
+    · simp
+
+theorem Ty.spine_ren_none {R : Ty} (r : Ren Ty)
+  : R.spine = none -> R⟨r⟩.spine = none
+:= by
+  intro h
+  induction R <;> simp [spine] at *
+  case _ f _ ih _ =>
+    rw[quantifier_bundle, option_lemma] at *
+    apply ih h
+
+def Ty.is_all_some : Ty -> Option (Kind × Ty)
+| .all K B => return (K, B)
+| _ => none
+
+def Ty.is_all_some_sound {T : Ty} :
+  T.is_all_some = .some (K, T1) ->
+  T = `∀[K] T1 := by
+intro h
+cases T <;> simp [Ty.is_all_some] at *
+assumption
+
+def Ty.is_then_some : Ty -> Option (Ty × Ty)
+| A `=:> B => return (A, B)
+| _ => none
+
+def Ty.is_arrow_some_sound {T : Ty} :
+  T.is_then_some = .some (T1, T2) ->
+  T = T1 `=:> T2 := by
+intro h
+cases T <;> simp [Ty.is_then_some] at *
+assumption
+
+def Ty.is_app_some : Ty -> Option (Ty × Ty)
+| .app A B => return (A, B)
+| _ => none
+
+def Ty.is_app_some_sound {T : Ty} :
+  T.is_app_some = some (A, B) ->
+  T = (A `• B) := by
+intro h;
+cases T <;> simp [Ty.is_app_some] at *
+assumption
+
+def Ty.subterms : Ty -> List Ty
+| .app x y => x.subterms ++ y.subterms ++ [.app x y]
+| .arrow x y => x.subterms ++ y.subterms ++ [.arrow x y]
+| .then x y => x.subterms ++ y.subterms ++ [.then x y]
+| x => [x]
 
 
-def Surface.Ty.overloaded_type : Surface.Ty -> (List Surface.Ty × Surface.Ty)
-| .then A B =>
-  let (is, y) := Surface.Ty.overloaded_type B
-  ((A :: is), y)
-| B => ([], B)
+end Surface
