Surface/Ty/Substitution.lean
@@ -1,144 +1,201 @@
 import LeanSubst
+import Lilac
 import Surface.Ty.Definition
 
 open LeanSubst
+open Lilac
 
-
+namespace Surface
 @[coe]
-def Surface.Ty.from_action : Subst.Action Surface.Ty -> Surface.Ty
+def Ty.from_action : Action Ty -> Ty
 | .re y => t`#y
 | .su t => t
 
 @[simp]
-theorem Surface.Ty.from_action_id {n} : from_action (+0 n) = t`#n := by
+theorem Ty.from_action_id {n} : from_action (+0σ.act n) = t`#n := by
   simp [from_action, Subst.id]
 
 @[simp]
-theorem Surface.Ty.from_action_succ {n} : from_action (+1 n) = t`#(n + 1) := by
+theorem Ty.from_action_succ {n} : from_action (+1σ.act n) = t`#(n + 1) := by
   simp [from_action, Subst.succ]
 
 @[simp]
-theorem Surface.Ty.from_acton_re {n} : from_action (re n) = t`#n := by simp [from_action]
+theorem Ty.from_acton_re {n} : from_action (re n) = t`#n := by simp [from_action]
 
 @[simp]
-theorem Surface.Ty.from_action_su {t} : from_action (su t) = t := by simp [from_action]
+theorem Ty.from_action_su {t} : from_action (su t) = t := by simp [from_action]
 
-instance Surface.Coe_ActionTyTy : Coe (Subst.Action Surface.Ty) Surface.Ty where
-  coe := Surface.Ty.from_action
+instance : Coe (Action Ty) Ty where
+  coe := Ty.from_action
+
 
 @[simp]
-def Surface.Ty.rmap (r : Ren) : Ty -> Ty
-| t`#x => t`#(r x)
+def Ty.rmap (r : Ren Ty) : Ty -> Ty
+| t`#x => t`#(r.act x)
 | gt`#x => gt`#x
 | A `-:> B => rmap r A `-:> rmap r B
 | A `=:> B => rmap r A `=:> rmap r B
 | `∀[K] P => `∀[K] rmap r.lift P
-| app f a => rmap r f `• rmap r a
+| .app f a => rmap r f `• rmap r a
 
-instance Surface.instRenMap_SurfaceTy : RenMap Surface.Ty where
+instance instRenMap_SurfaceTy : RenMap Ty Ty where
   rmap := Surface.Ty.rmap
 
 @[simp]
-def Surface.Ty.smap (σ : Subst Surface.Ty) : Surface.Ty -> Surface.Ty
-| t`#x => σ x
+theorem Ty.ren_var {r : Ren Ty} : (t`#x)⟨r⟩ = t`#(r.act x) := by
+  simp [RenMap.rmap]
+
+@[simp]
+theorem Ty.ren_global {r : Ren Ty} : (gt`#x)⟨r⟩ = gt`#x := by
+  simp [RenMap.rmap]
+
+@[simp]
+theorem Ty.ren_arr {A B : Ty} {r : Ren Ty} : (A `-:> B)⟨r⟩ = A⟨r⟩ `-:> B⟨r⟩ := by
+  simp [RenMap.rmap]
+
+@[simp]
+theorem Ty.ren_then {A B : Ty} {r : Ren Ty} : (A `=:> B)⟨r⟩ = A⟨r⟩ `=:> B⟨r⟩ := by
+  simp [RenMap.rmap]
+
+@[simp]
+theorem Ty.ren_all {r : Ren Ty} : (`∀[K] P)⟨r⟩ = `∀[K] P⟨r.lift⟩ := by
+  simp [RenMap.rmap]
+
+@[simp]
+theorem Ty.ren_app {r : Ren Ty} : (f `• a)⟨r⟩ = f⟨r⟩ `• a⟨r⟩ := by
+  simp [RenMap.rmap]
+
+
+instance : RenMapId Ty Ty where
+  apply_id := by subst_solve_id
+
+instance : RenMapCompose Ty Ty where
+  apply_compose := by subst_solve_compose
+
+
+@[simp]
+def Ty.smap (σ : Subst Ty) : Ty -> Ty
+| t`#x => σ.act x
 | gt`#x => gt`#x
 | A `-:> B => smap σ A `-:> smap σ B
 | A `=:> B => smap σ A `=:> smap σ B
 | `∀[K] P => `∀[K] smap σ.lift P
-| app f a => smap σ f `• smap σ a
+| .app f a => smap σ f `• smap σ a
 
-instance Surface.instSubstMap_TyTy : SubstMap Surface.Ty Surface.Ty where
+instance instSubstMap_TyTy : SubstMap Surface.Ty Surface.Ty where
   smap := Surface.Ty.smap
 
 @[simp]
-theorem Surface.Ty.subst_var : (t`#x)[σ:Ty] = σ x := by
+theorem Ty.subst_var {σ : Subst Ty}: (t`#x)[σ] = σ.act x := by
   simp [SubstMap.smap]
 
 @[simp]
-theorem Surface.Ty.subst_global : (gt`#x)[σ:Ty] = gt`#x := by
+theorem Ty.subst_global {σ : Subst Ty}: (gt`#x)[σ] = gt`#x := by
   simp [SubstMap.smap]
 
 @[simp]
-theorem Surface.Ty.subst_arr {A B : Ty} : (A `-:> B)[σ:Ty] = A[σ:_] `-:> B[σ:_] := by
+theorem Ty.subst_arr {σ : Subst Ty}{A B : Ty} : (A `-:> B)[σ] = A[σ] `-:> B[σ] := by
   simp [SubstMap.smap]
 
 @[simp]
-theorem Surface.Ty.subst_then {A B : Ty} : (A `=:> B)[σ:Ty] = A[σ:_] `=:> B[σ:_] := by
+theorem Ty.subst_then {σ : Subst Ty} {A B : Ty} : (A `=:> B)[σ] = A[σ] `=:> B[σ] := by
   simp [SubstMap.smap]
 
 @[simp]
-theorem Surface.Ty.subst_all : (`∀[K] P)[σ:Ty] = `∀[K] P[σ.lift:_] := by
+theorem Ty.subst_all {σ : Subst Ty} : (`∀[K]P)[σ] = `∀[K] P[σ.lift] := by
   simp [SubstMap.smap]
 
 @[simp]
-theorem Surface.Ty.subst_app : (f `• a)[σ:Ty] = f[σ:_] `• a[σ:_] := by
+theorem Ty.subst_app {σ : Subst Ty} : (f `• a)[σ] = f[σ] `• a[σ] := by
   simp [SubstMap.smap]
 
 @[simp]
-theorem Surface.Ty.from_action_compose {x} {σ τ : Subst Ty}
-  : (from_action (σ x))[τ] = from_action ((σ ∘ τ) x)
+theorem Ty.from_action_compose {x : Nat} {σ τ : Subst Ty}
+  : (from_action (σ.act x))[τ] = from_action ((σ ∘ τ).act x)
 := by
   simp [Ty.from_action, Subst.compose]
-  generalize zdef : σ x = z
+  generalize zdef : σ.act x = z
   cases z <;> simp [Ty.from_action]
 
-theorem Surface.Ty.apply_id {t : Surface.Ty} : t[+0] = t := by
-  induction t; all_goals (simp at *; try simp [*])
-
-instance Surface.instSubstMapId_TyTy: SubstMapId Surface.Ty Surface.Ty where
-  apply_id := Surface.Ty.apply_id
-
-theorem Surface.Ty.apply_stable (r : Ren) (σ : Subst Surface.Ty)
-  : r.to = σ -> rmap r = smap σ
-:= by subst_solve_stable r, σ
-
-instance Surface.instSubstMapStable_Ty: SubstMapStable Surface.Ty where
-  apply_stable := Surface.Ty.apply_stable
-
-theorem Surface.Ty.apply_compose {s : Ty} {σ τ : Subst Ty} : s[σ][τ] = s[σ ∘ τ] := by
-  subst_solve_compose Ty, s, σ, τ
-
-instance Surface.instSubstMapCompose_TyTy : SubstMapCompose Surface.Ty Surface.Ty where
-  apply_compose := Surface.Ty.apply_compose
-
-theorem Surface.Ty.rename_preserves_var_shape {r : Ren} : t`#x = T[r] -> ∃ y,  (T = t`#y ∧ x = r y) := by
-intro h
-induction T <;> simp at *
-case var => simp [Ren.to] at h; assumption
-
-
-theorem Surface.Ty.rename_preserves_global_shape {r : Ren} : gt`#x = T[r] -> T = gt`#x := by
-intro h
-induction T <;> simp at *
-case var => simp [Ren.to] at h
-case global => symm at h; assumption
-
-
-theorem Surface.Ty.rename_preserves_arrow_shape {A B : Ty}{r : Ren} : A `-:> B = T[r] ->
-  (∃ A' B' : Ty, (T = A' `-:> B') ∧  A = A'[r] ∧ B = B'[r])
+@[simp]
+theorem Ty.from_action_compose_ren {x : Nat} {σ : Subst Ty} {r : Ren Ty}
+  : (from_action (σ.act x))⟨r⟩ = from_action ((σ ∘ r).act x)
 := by
-intro h
-induction T <;> simp at *
-case var => simp [Ren.to] at h
-case arrow a1 a2 _ _ => exists a1; exists a2
+  simp [Ty.from_action]
+  generalize zdef : σ.act x = z
+  cases z <;> simp
 
-theorem Surface.Ty.rename_preserves_app_shape {A B : Ty}{r : Ren} : (A `• B) = T[r] ->
-  (∃ A' B' : Ty, (T = A' `• B') ∧  A = A'[r] ∧ B = B'[r])
+instance instSubstMapId_TyTy: SubstMapId Surface.Ty Surface.Ty where
+  apply_id := by subst_solve_id
+
+instance instSubstMapStableTyTy : SubstMapStable Ty Ty where
+  apply_stable := by
+    intro r σ h; funext; case _ t =>
+    induction t generalizing r σ
+      <;> simp [-Subst.rewrite_lift, -Subst.rewrite_lift_ren, -Subst.rewrite_lift_k_ren, *]
+    case var => rw [<-h]; simp
+
+instance : SubstMapRenComposeLeft Ty Ty where
+  apply_ren_compose_left := by subst_solve_compose
+
+instance : SubstMapRenComposeRight Ty Ty where
+  apply_ren_compose_right := by subst_solve_compose
+
+instance : SubstMapCompose Ty Ty where
+  apply_compose := by subst_solve_compose
+
+@[simp]
+def SpineTy.rmap (r : Ren Ty) : SpineTy -> SpineTy
+| ⟨m1, Ks1, m2, Ks2, n, Ts, R⟩ =>
+  ⟨m1, Ks1, m2, Ks2, n, Vec.map (·⟨r.lift (m1 + m2)⟩) Ts, R⟨r.lift (m1 + m2)⟩⟩
+
+instance : RenMap SpineTy Ty where
+  rmap := SpineTy.rmap
+
+@[simp]
+theorem SpineTy.rmap_eq {r : Ren Ty}
+  : (⟨m1, Ks1, m2, Ks2, n, Ts, R⟩ : SpineTy)⟨r⟩
+    = ⟨m1, Ks1, m2, Ks2, n, Ts⟨r.lift (m1 + m2)⟩, R⟨r.lift (m1 + m2)⟩⟩
 := by
-intro h
-induction T <;> simp at *
-case var => simp [Ren.to] at h
-case app a1 a2 _ _  =>
-  cases h.1; cases h.2; clear h
-  exists a1; exists a2
+  simp [RenMap.rmap]
+  induction Ts <;> simp [Vec.rmap, *, RenMap.rmap]
 
+@[simp]
+def SpineTy.smap (σ : Subst Ty) : SpineTy -> SpineTy
+| ⟨m1, Ks1, m2, Ks2, n, Ts, R⟩ =>
+  ⟨m1, Ks1, m2, Ks2, n, Vec.map (·[σ.lift (m1 + m2)]) Ts, R[σ.lift (m1 + m2)]⟩
 
-theorem Surface.Ty.rename_preserves_all_shape {P : Ty}{r : Ren} : (`∀[K] P) = T[r] ->
-  (∃ P' : Ty, (T = `∀[K]P') ∧  P = P'[re 0::↑r ∘ +1:Ty])
+instance : SubstMap SpineTy Ty where
+  smap := SpineTy.smap
+
+@[simp]
+theorem SpineTy.smap_eq {σ : Subst Ty}
+  : (⟨m1, Ks1, m2, Ks2, n, Ts, R⟩ : SpineTy)[σ]
+    = ⟨m1, Ks1, m2, Ks2, n, Ts[σ.lift (m1 + m2)], R[σ.lift (m1 + m2)]⟩
 := by
-intro h
-induction T generalizing K P <;> simp at *
-case var => simp [Ren.to] at h
-case all a ih =>
-  cases h.1; cases h.2; clear h
-  exists a;
+  simp [SubstMap.smap]
+  induction Ts <;> simp [Vec.smap, *, SubstMap.smap]
+
+instance : SubstMapId SpineTy Ty where
+  apply_id := by intro t; rcases t with ⟨m1, Ks1, m2, Ks2, n, Ts, R⟩; simp
+
+instance : SubstMapRenComposeLeft SpineTy Ty where
+  apply_ren_compose_left := by
+    intro t; rcases t with ⟨m1, Ks1, m2, Ks2, n, Ts, R⟩
+    simp [-Subst.rewrite_lift_k_ren, -Subst.rewrite_lift_k]
+
+instance : SubstMapRenComposeRight SpineTy Ty where
+  apply_ren_compose_right := by
+    intro t; rcases t with ⟨m1, Ks1, m2, Ks2, n, Ts, R⟩
+    simp [-Subst.rewrite_lift_k_ren, -Subst.rewrite_lift_k]
+
+instance : SubstMapCompose SpineTy Ty where
+  apply_compose := by
+    intro t; rcases t with ⟨m1, Ks1, m2, Ks2, n, Ts, R⟩
+    simp [-Subst.rewrite_lift_k_ren, -Subst.rewrite_lift_k]
+
+theorem Ty.rmap_promote : Ty.rmap r A = A⟨r⟩ := by simp [RenMap.rmap]
+
+theorem Ty.smap_promote : Ty.smap σ A = A[σ] := by simp [SubstMap.smap]
+
+end Surface
