Core/Ppcc/Lemmas.lean
@@ -13,4 +13,65 @@ theorem EqGraph.ask_type_sound {G : GlobalEnv} {wf : ⊢ G} {Δ : KindEnv} {Γ :
 
 
 
+
+theorem EqGraph.push_preserves_wf {G : GlobalEnv} {Δ : KindEnv} {Γ : TyEnv}
+  {n : Node G Δ} {eG eG' : EqGraph G Δ Γ} (wf : eG.Wf) :
+  eG.push n = eG' ->
+  eG'.Wf
+:= by sorry
+-- intro h; unfold Wf at wf
+-- unfold push at h;
+-- split at h
+-- · subst h; assumption
+-- · simp only [<-h, Wf]; simp
+
+
+theorem EqGraph.union_equiv_class_count {G : GlobalEnv} {wf : ⊢ G} {Δ : KindEnv} {Γ : TyEnv}
+  {eG eG' : EqGraph G Δ Γ} {K : Kind}
+  {T1 : Ty} {T2 : Ty} {t : Term} {j : G&Δ, Γ ⊢ t : (T1 ~[K]~ T2)} (inv : eG.equiv_class_count > 0):
+  eG.union (wf := wf) K T1 T2 t j = some eG' ->
+  eG'.equiv_class_count < eG.equiv_class_count
+  := by
+  intro h
+  unfold EqGraph.union at h; simp at h
+  rw[Option.bind_eq_some_iff] at h; rcases h with ⟨i1, h1, h⟩
+  rw[Option.bind_eq_some_iff] at h; rcases h with ⟨i2, h2, h⟩
+  split at h
+  · rw[Option.bind_eq_some_iff] at h; rcases h with ⟨⟨ip1, pT1, K1, _, _⟩, h3, h⟩
+    rw[Option.bind_eq_some_iff] at h; rcases h with ⟨⟨ip2, pT2, K2, _, _⟩, h4, h⟩
+    simp at h
+    split at h
+    · simp at h;
+      rcases h with ⟨ne, h⟩
+      split at h <;> simp at h
+      · rw[<-h]; simp; omega
+      · rcases h with ⟨_, h⟩; rw[<-h]; simp; omega
+    · cases h
+  · cases h
+
+
+theorem EqGraph.union_preserves_wf
+{G : GlobalEnv} {wfg : ⊢ G} {Δ : KindEnv} {Γ : TyEnv}
+  {K : Kind} {T1 T2 : Ty} {t : Term} {j : G&Δ, Γ ⊢ t : (T1 ~[K]~ T2)} {eG eG' : EqGraph G Δ Γ}
+  (wf : eG.Wf) :
+  eG.union wfg K T1 T2 t j = some eG' ->
+  eG'.Wf
+:= by
+intro h
+unfold union at h; simp at h
+rw[Option.bind_eq_some_iff] at h; rcases h with ⟨i1, h1, h⟩
+rw[Option.bind_eq_some_iff] at h; rcases h with ⟨i2, h2, h⟩
+split at h
+case _ h3 h4 =>
+  rw[Option.bind_eq_some_iff] at h; rcases h with ⟨rep_T1, h5, h⟩
+  rw[Option.bind_eq_some_iff] at h; rcases h with ⟨rep_T2, h6, h⟩
+  split at h
+  case _ h7 h8 =>
+    simp at h; rcases h with ⟨h9, h⟩
+    split at h
+    case _ h10 => simp at h; simp only [<-h, Wf]; simp; sorry
+    sorry
+  case _ => cases h
+case _ => cases h
+
 end Core.Ppcc
