Surface/Ty/BEq.lean
@@ -1,56 +1,58 @@
 import Surface.Ty.Definition
 
-def Surface.BaseKind.beq : Surface.BaseKind -> Surface.BaseKind -> Bool
+namespace Surface
+
+def BaseKind.beq : Surface.BaseKind -> Surface.BaseKind -> Bool
 | closed, closed => true
 | .open, .open => true
 | _, _ => false
 
 
-instance Surface.instBEq_BaseKind : BEq BaseKind where
+instance instBEq_BaseKind : BEq BaseKind where
   beq := Surface.BaseKind.beq
 
 @[simp]
-instance Surface.instReflBEq_BaseKind : ReflBEq Surface.BaseKind where
+instance instReflBEq_BaseKind : ReflBEq Surface.BaseKind where
   rfl := by
     intro a
     cases a
-    all_goals (simp [Surface.instBEq_BaseKind, Surface.BaseKind.beq])
+    all_goals (simp +instances [Surface.instBEq_BaseKind, Surface.BaseKind.beq])
 
 @[simp]
-instance Surface.instLawfulBEq_BaseKind : LawfulBEq Surface.BaseKind where
+instance instLawfulBEq_BaseKind : LawfulBEq Surface.BaseKind where
   eq_of_beq := by
     intro a b h
     cases a <;> cases b
     all_goals (simp at *)
-    all_goals (simp [instBEq_BaseKind, BaseKind.beq] at h)
+    all_goals (simp +instances [instBEq_BaseKind, BaseKind.beq] at h)
 
-def Surface.Kind.beq : Kind -> Kind -> Bool
+def Kind.beq : Kind -> Kind -> Bool
 | base b1, base b2 => b1 == b2
 | arrow A1 B1, arrow A2 B2 => Kind.beq A1 A2 && Kind.beq B1 B2
 | _, _ => false
 
 
-instance Surface.instBEq_Kind : BEq Kind where
+instance instBEq_Kind : BEq Kind where
   beq := Kind.beq
 
 
-instance Surface.instReflBEq_Kind : ReflBEq Kind where
+instance instReflBEq_Kind : ReflBEq Kind where
   rfl := by
-    intro a; induction a <;> simp [Kind.beq, instBEq_Kind] at *
+    intro a; induction a <;> simp +instances [Kind.beq, instBEq_Kind] at *
     case _ ih1 ih2 =>
     constructor; apply ih1; apply ih2
 
-instance Surface.instLawfulBeq_Kind : LawfulBEq Kind where
+instance instLawfulBeq_Kind : LawfulBEq Kind where
   eq_of_beq := by
     intro a b h
-    induction a, b using Kind.beq.induct <;> simp [instBEq_Kind, Kind.beq] at *
+    induction a, b using Kind.beq.induct <;> simp +instances [instBEq_Kind, Kind.beq] at *
     apply h
     case _ ih1 ih2 =>
       constructor
       · apply ih1 h.1
       · apply ih2 h.2
 
-def Surface.Ty.beq : Ty -> Ty -> Bool
+def Ty.beq : Ty -> Ty -> Bool
 | var x, var y => x == y
 | global x, global y => x == y
 | arrow A1 B1, arrow A2 B2 => beq A1 A2 && beq B1 B2
@@ -59,19 +61,19 @@ def Surface.Ty.beq : Ty -> Ty -> Bool
 | app A1 B1, app A2 B2 => beq A1 A2 && beq B1 B2
 | _, _ => false
 
-instance Surface.instBEq_Ty : BEq Ty where
+instance instBEq_Ty : BEq Ty where
   beq := Ty.beq
 
-instance Surface.instReflBEq_Type : ReflBEq Ty where
+instance instReflBEq_Type : ReflBEq Ty where
   rfl := by
-    intro a; induction a <;> simp [instBEq_Ty, Ty.beq] at *
+    intro a; induction a <;> simp +instances [instBEq_Ty, Ty.beq] at *
     all_goals (try case _ ih1 ih2 => constructor; assumption; assumption)
     case _ => assumption
 
-instance Surface.instLawfulBeq_Ty : LawfulBEq Ty where
+instance instLawfulBeq_Ty : LawfulBEq Ty where
   eq_of_beq := by
     intro a b h
-    induction a, b using Surface.Ty.beq.induct <;> simp [Surface.instBEq_Ty, Surface.Ty.beq] at *
+    induction a, b using Surface.Ty.beq.induct <;> simp +instances [Surface.instBEq_Ty, Surface.Ty.beq] at *
     assumption
     assumption
     all_goals (try
@@ -83,3 +85,5 @@ instance Surface.instLawfulBeq_Ty : LawfulBEq Ty where
       constructor
       · apply h.1
       · apply ih h.2
+
+end Surface
